theories/language/metatheory.v
@@ -31,7 +31,7 @@ Fixpoint expr_closed X e :=
   | Constr _ e
   | Fork e
   | Load e =>
-     expr_closed X e
+      expr_closed X e
   | App e1 e2
   | Binop _ e1 e2
   | Equal e1 e2
@@ -40,12 +40,14 @@ Fixpoint expr_closed X e :=
   | Store e1 e2
   | Xchg e1 e2
   | Faa e1 e2 =>
-     expr_closed X e1 && expr_closed X e2
+      expr_closed X e1 && expr_closed X e2
   | If e0 e1 e2
   | Case e0 e1 e2
   | Cas e0 e1 e2
   | Resolve e0 e1 e2 =>
-     expr_closed X e0 && expr_closed X e1 && expr_closed X e2
+      expr_closed X e0 && expr_closed X e1 && expr_closed X e2
+  | Record es =>
+      forallb (expr_closed X) es
   | Proph =>
       true
   end
@@ -68,11 +70,11 @@ Fixpoint subst_map (vs : gmap string val) e :=
   | Var y =>
       if vs !! y is Some v then Val v else Var y
   | Rec f y e =>
-      Rec f y (subst_map (binder_delete y (binder_delete f vs)) e)
+      Rec f y $ subst_map (binder_delete y (binder_delete f vs)) e
   | App e1 e2 =>
       App (subst_map vs e1) (subst_map vs e2)
   | Unop op e =>
-      Unop op (subst_map vs e)
+      Unop op $ subst_map vs e
   | Binop op e1 e2 =>
       Binop op (subst_map vs e1) (subst_map vs e2)
   | Equal e1 e2 =>
@@ -82,19 +84,21 @@ Fixpoint subst_map (vs : gmap string val) e :=
   | Pair e1 e2 =>
       Pair (subst_map vs e1) (subst_map vs e2)
   | Fst e =>
-      Fst (subst_map vs e)
+      Fst $ subst_map vs e
   | Snd e =>
-      Snd (subst_map vs e)
+      Snd $ subst_map vs e
   | Constr b e =>
-      Constr b (subst_map vs e)
+      Constr b $ subst_map vs e
   | Case e0 e1 e2 =>
       Case (subst_map vs e0) (subst_map vs e1) (subst_map vs e2)
   | Fork e =>
-      Fork (subst_map vs e)
+      Fork $ subst_map vs e
+  | Record es =>
+      Record $ subst_map vs <$> es
   | Alloc e1 e2 =>
       Alloc (subst_map vs e1) (subst_map vs e2)
   | Load e =>
-      Load (subst_map vs e)
+      Load $ subst_map vs e
   | Store e1 e2 =>
       Store (subst_map vs e1) (subst_map vs e2)
   | Xchg e1 e2 =>
@@ -116,14 +120,16 @@ Proof.
   destruct 1; constructor; destruct x; set_solver.
 Qed.
 
-Lemma subst_closed X e x es :
+Lemma subst_closed X e x v :
   expr_closed X e →
   x ∉ X →
-  subst x es e = e.
+  subst x v e = e.
 Proof.
-  revert X. induction e=> X /=;
+  move: X. induction e => X /=;
     rewrite ?bool_decide_spec ?andb_True => ? ?;
     repeat case_decide; simplify_eq/=; f_equal; intuition eauto with set_solver.
+  select (Forall _ _) ltac:(fun H => induction H; first done).
+  rewrite fmap_cons. f_equal; naive_solver.
 Qed.
 
 Lemma subst_closed_empty e x v :
@@ -136,8 +142,10 @@ Qed.
 Lemma subst_subst e x v v' :
   subst x v (subst x v' e) = subst x v' e.
 Proof.
-  intros. induction e; simpl; try (f_equal; by auto);
+  intros. induction e; simpl; try (f_equal; auto; done);
     simplify_option_eq; auto using subst_closed_empty with f_equal.
+  select (Forall _ _) ltac:(fun H => induction H; first done).
+  rewrite !fmap_cons. do 2 f_equal; naive_solver.
 Qed.
 Lemma subst_subst' e x v v' :
   subst' x v (subst' x v' e) = subst' x v' e.
@@ -151,6 +159,8 @@ Lemma subst_subst_ne e x y v v' :
 Proof.
   intros. induction e; simpl; try (f_equal; by auto);
     simplify_option_eq; auto using eq_sym, subst_closed_empty with f_equal.
+  select (Forall _ _) ltac:(fun H => induction H; first done).
+  rewrite !fmap_cons. do 2 f_equal; naive_solver.
 Qed.
 Lemma subst_subst_ne' e x y v v' :
   x ≠ y →
