theories/language/tactics.v
@@ -11,80 +11,106 @@ From zebre Require Import
 Create HintDb zebre.
 
 Ltac reshape_expr e tac :=
-  let rec go K vs e :=
+  let rec go K pvs e :=
     match e with
     | _ =>
-        lazymatch vs with
-        | [] =>
+        lazymatch pvs with
+        | nil =>
             tac K e
         | _ =>
             fail
         end
     | App ?e1 (Val ?v2) =>
-        add_ectxi (CtxAppL v2) vs K e1
+        add_ectxi (CtxAppL v2) K pvs e1
     | App ?e1 ?e2 =>
-        add_ectxi (CtxAppR e1) vs K e2
+        add_ectxi (CtxAppR e1) K pvs e2
     | Unop ?op ?e =>
-        add_ectxi (CtxUnop op) vs K e
+        add_ectxi (CtxUnop op) K pvs e
     | Binop ?op ?e1 (Val ?v2) =>
-        add_ectxi (CtxBinopL op v2) vs K e1
+        add_ectxi (CtxBinopL op v2) K pvs e1
     | Binop ?op ?e1 ?e2 =>
-        add_ectxi (CtxBinopR op e1) vs K e2
+        add_ectxi (CtxBinopR op e1) K pvs e2
     | Equal ?e1 (Val ?v2) =>
-        add_ectxi (CtxEqualL v2) vs K e1
+        add_ectxi (CtxEqualL v2) K pvs e1
     | Equal ?e1 ?e2 =>
-        add_ectxi (CtxEqualR e1) vs K e2
+        add_ectxi (CtxEqualR e1) K pvs e2
     | If ?e0 ?e1 ?e2 =>
-        add_ectxi (CtxIf e1 e2) vs K e0
+        add_ectxi (CtxIf e1 e2) K pvs e0
     | Pair ?e1 (Val ?v2) =>
-        add_ectxi (CtxPairL v2) vs K e1
+        add_ectxi (CtxPairL v2) K pvs e1
     | Pair ?e1 ?e2 =>
-        add_ectxi (CtxPairR e1) vs K e2
+        add_ectxi (CtxPairR e1) K pvs e2
     | Fst ?e =>
-        add_ectxi CtxFst vs K e
+        add_ectxi CtxFst K pvs e
     | Snd ?e =>
-        add_ectxi CtxSnd vs K e
+        add_ectxi CtxSnd K pvs e
     | Constr ?b ?e =>
-        add_ectxi (CtxConstr b) vs K e
+        add_ectxi (CtxConstr b) K pvs e
     | Case ?e0 ?e1 ?e2 =>
-        add_ectxi (CtxCase e1 e2) vs K e0
+        add_ectxi (CtxCase e1 e2) K pvs e0
+    | Record ?es =>
+        go_list K pvs CtxRecord es
     | Alloc ?e1 (Val ?v2) =>
-        add_ectxi (CtxAllocL v2) vs K e1
+        add_ectxi (CtxAllocL v2) K pvs e1
     | Alloc ?e1 ?e2 =>
-        add_ectxi (CtxAllocR e1) vs K e2
+        add_ectxi (CtxAllocR e1) K pvs e2
     | Load ?e =>
-        add_ectxi CtxLoad vs K e
+        add_ectxi CtxLoad K pvs e
     | Store ?e1 (Val ?v2) =>
-        add_ectxi (CtxStoreL v2) vs K e1
+        add_ectxi (CtxStoreL v2) K pvs e1
     | Store ?e1 ?e2 =>
-        add_ectxi (CtxStoreR e1) vs K e2
+        add_ectxi (CtxStoreR e1) K pvs e2
     | Xchg ?e1 (Val ?v2) =>
-        add_ectxi (CtxXchgL v2) vs K e1
+        add_ectxi (CtxXchgL v2) K pvs e1
     | Xchg ?e1 ?e2 =>
-        add_ectxi (CtxXchgR e1) vs K e2
+        add_ectxi (CtxXchgR e1) K pvs e2
     | Cas ?e0 (Val ?v1) (Val ?v2) =>
-        add_ectxi (CtxCasL v1 v2) vs K e0
+        add_ectxi (CtxCasL v1 v2) K pvs e0
     | Cas ?e0 ?e1 (Val ?v2) =>
-        add_ectxi (CtxCasM e0 v2) vs K e1
+        add_ectxi (CtxCasM e0 v2) K pvs e1
     | Cas ?e0 ?e1 ?e2 =>
-        add_ectxi (CtxCasR e0 e1) vs K e2
+        add_ectxi (CtxCasR e0 e1) K pvs e2
     | Faa ?e1 (Val ?v2) =>
-        add_ectxi (CtxFaaL v2) vs K e1
+        add_ectxi (CtxFaaL v2) K pvs e1
     | Faa ?e1 ?e2 =>
-        add_ectxi (CtxFaaR e1) vs K e2
+        add_ectxi (CtxFaaR e1) K pvs e2
     | Resolve ?e0 (Val ?v1) (Val ?v2) =>
-        go K ((v1, v2) :: vs) e0
+        go K (cons (v1, v2) pvs) e0
     | Resolve ?e0 ?e1 (Val ?v2) =>
-        add_ectxi (CtxResolveM e0 v2) vs K e1
+        add_ectxi (CtxResolveM e0 v2) K pvs e1
     | Resolve ?e0 ?e1 ?e2 =>
-        add_ectxi (CtxResolveR e0 e1) vs K e2
+        add_ectxi (CtxResolveR e0 e1) K pvs e2
     end
-  with add_ectxi k vs K e :=
-    lazymatch vs with
-    | [] =>
-        go (k :: K) (@nil (val * val)) e
-    | (?v1, ?v2) :: ?vs =>
-        add_ectxi (CtxResolveL k v1 v2) vs K e
+  with go_list K pvs ctx es :=
+    go_list' K pvs ctx (@nil val) es
+  with go_list' K pvs ctx vs es :=
+    lazymatch es with
+    | cons ?e ?es =>
+        lazymatch e with
+        | Val ?v =>
+            go_list' K pvs ctx (cons v vs) es
+        | _ =>
+            go_list'' K pvs ctx vs e es
+        end
+    | _ =>
+        fail
+    end
+  with go_list'' K pvs ctx vs e es :=
+    first
+    [ add_ectxi (ctx (rev vs) es) K pvs e
+    | lazymatch vs with
+      | nil =>
+          fail
+      | cons ?v ?vs =>
+          go_list'' K pvs ctx vs (Val v) (cons e es)
+      end
+    ]
+  with add_ectxi k K pvs e :=
+    lazymatch pvs with
+    | nil =>
+        go (cons k K) (@nil (val * val)) e
+    | cons (?v1, ?v2) ?pvs =>
+        add_ectxi (CtxResolveL k v1 v2) K pvs e
     end
   in
   go (@nil ectxi) (@nil (val * val)) e.
@@ -125,6 +151,11 @@ Ltac invert_head_step :=
   head_step (Equal _ _) _ _ _ _ _
 ) =>
   eapply head_step_equal_suc
+: zebre.
+#[global] Hint Extern 0 (
+  head_step (Record  _) _ _ _ _ _
+) =>
+  eapply head_step_record'
 : zebre.
 #[global] Hint Extern 0 (
   head_step (Alloc _ _) _ _ _ _ _
