theories/persistent/parray.v
@@ -4,7 +4,6 @@ From iris.base_logic Require Import
 From zebre Require Import
   prelude.
 From zebre.language Require Import
-  tactics
   notations
   diaframe.
 From zebre.std Require Import
