theories/std/safe_dynarray.v
@@ -12,7 +12,6 @@ From zebre.std Require Export
 From zebre.std Require Import
   diverge
   assume
-  record
   math
   reference
   opt
@@ -45,17 +44,17 @@ Implicit Types vs : list val.
 
 Definition safe_dynarray_create : val :=
   λ: <>,
-    record2 #0 (array_create #()).
+    { #0; array_create #() }.
 
 Definition safe_dynarray_make : val :=
   λ: "sz" "v",
     assume (#0 ≤ "sz") ;;
-    record2 "sz" (array_initi "sz" (λ: <>, &Some (ref "v"))).
+    { "sz"; array_initi "sz" (λ: <>, &Some (ref "v")) }.
 
 Definition safe_dynarray_initi : val :=
   λ: "sz" "fn",
     assume (#0 ≤ "sz") ;;
-    record2 "sz" (array_initi "sz" (λ: "i", &Some (ref ("fn" "i")))).
+    { "sz"; array_initi "sz" (λ: "i", &Some (ref ("fn" "i"))) }.
 
 Definition safe_dynarray_size : val :=
   λ: "t",
@@ -199,7 +198,7 @@ Section zebre_G.
     iIntros "%Φ _ HΦ".
     wp_rec.
     wp_apply (array_create_spec with "[//]") as "%data Hdata_model".
-    wp_apply (record2_spec with "[//]") as "%l (_ & Hsz & Hdata)".
+    wp_record l as "(Hsz & Hdata & _)".
     iApply "HΦ". iExists l, data, [], 0. iSteps.
   Qed.
 
@@ -217,8 +216,8 @@ Section zebre_G.
     wp_rec.
     wp_smart_apply assume_spec' as "_".
     wp_smart_apply (array_initi_spec_disentangled (λ _ slot, slot_model slot v)) as "%data %slots (%Hslots & Hdata_model & Hslots)"; [done | iSteps |].
-    wp_apply (record2_spec with "[//]") as "%l (_ & Hsz & Hdata)".
-    iApply "HΦ". iExists l, data, slots, 0. iFrame. iSplit; first iSteps.
+    wp_record l as "(Hsz & Hdata & _)".
+    iApply "HΦ". iExists l, data, slots, 0. iFrame. iSplitR; first iSteps.
     rewrite replicate_length right_id. iFrame.
     iApply (big_sepL2_replicate_r_2 _ _ (λ _, slot_model) with "Hslots"). lia.
   Qed.
@@ -259,9 +258,9 @@ Section zebre_G.
       wp_alloc r as "Hr". wp_pures.
       iExists (vs ++ [v]). iFrame. iSteps.
     }
-    wp_apply (record2_spec with "[//]") as "%l (_ & Hsz & Hdata)".
+    wp_record l as "(Hsz & Hdata & _)".
     iDestruct (big_sepL2_length with "Hslots") as %Hslots'.
-    iApply "HΦ". iFrame. iSplit; first iSteps.
+    iApply "HΦ". iFrame. iSplitR; first iSteps.
     iExists l, data, slots, 0. iFrame. iSplitR; first iSteps. iSplitL "Hsz"; first iSteps.
     rewrite right_id //.
   Qed.
@@ -687,8 +686,6 @@ Section zebre_G.
     iIntros "%Φ _ HΦ".
     wp_rec.
     wp_apply (array_create_type slot_type with "[//]") as "%data Hdata_type".
-    iApply wp_fupd.
-    wp_apply (record2_spec with "[//]") as "%l (_ & Hsz & Hdata)".
     iSteps.
   Qed.
 
@@ -707,8 +704,6 @@ Section zebre_G.
     wp_rec.
     wp_smart_apply assume_spec' as "%Hsz".
     wp_smart_apply (array_initi_type slot_type) as "%data (_ & Hdata_type)"; first iSteps.
-    iApply wp_fupd.
-    wp_smart_apply (record2_spec with "[//]") as "%l (_ & Hsz & Hdata)".
     iSteps.
   Qed.
 
